test/Test_Klas_GEMM_NaiveT__F32.cu
@@ -1,8 +1,0 @@
-#include "Klas_GEMM_NaiveT.h"
-
-#define stem         Klas_GEMM_NaiveT_g_matmul_
-#define et           float
-#define et_lbl       f32
-#define TOLERANCE    0.001f
-
-#include "normal_matmul_driver.c.inc"
