src/lib/kernel/gemm/Kuiper.Kernel.GEMM.Naive3.fst
@@ -3,11 +3,25 @@ module Kuiper.Kernel.GEMM.Naive3
 #set-options "--z3rlimit 20"
 
 #lang-pulse
+
 open Kuiper
-module T = Kuiper.Tensor
-module M = Kuiper.Array2
+open Kuiper.Tensor
+open Kuiper.Tensor { tensor_pts_to_cell as pts_to_cell }
 module MS = Kuiper.Spec.GEMM
-open Kuiper.EMatrix
+module SZ = Kuiper.SizeT
+open Kuiper.Index
+open Kuiper.Chest
+open Kuiper.Bijection
+open Kuiper.EMatrix { mkM, macc }
+
+let abs_bij (#m #n : nat)
+  : (abs (m @| n @| INil) =~ (natlt m & natlt n)) =
+  {
+    ff = (fun (i, (j, ())) -> (i, j));
+    gg = (fun (i, j) -> (i, (j, ())));
+    ff_gg = ez;
+    gg_ff = ez;
+  }
 
 unfold
 let kpre
@@ -15,26 +29,27 @@ let kpre
   (comb : binop et)
   (comb_r : binop real { comb `approx2` comb_r })
   (#m #n #k : nat)
-  (#lA : M.layout m k)
-  (#lB : M.layout k n)
-  (#lC : M.layout m n)
-  (gA : M.array2 et lA)
-  (gB : M.array2 et lB)
-  (gC : M.array2 et lC)
-  (eA : ematrix et m k)
-  (eB : ematrix et k n)
-  (eC : ematrix et m n)
-  (rA : ematrix real m k{eA %~ rA})
-  (rB : ematrix real k n{eB %~ rB})
-  (rC : ematrix real m n{eC %~ rC})
+  (#lA : layout2 m k)
+  (#lB : layout2 k n)
+  (#lC : layout2 m n)
+  (gA : tensor et lA)
+  (gB : tensor et lB)
+  (gC : tensor et lC)
+  (eA : chest2 et m k)
+  (eB : chest2 et k n)
+  (eC : chest2 et m n)
+  (rA : chest2 real m k{eA %~ rA})
+  (rB : chest2 real k n{eB %~ rB})
+  (rC : chest2 real m n{eC %~ rC})
   (fA fB : perm)
   (gid : natlt (m * n))
   : slprop
   =
   gA |-> Frac (fA /. (m * n)) eA **
   gB |-> Frac (fB /. (m * n)) eB **
-  M.pts_to_cell gC (gid / n, gid % n)
-    (macc eC (gid / n) (gid % n))
+  pts_to_cell gC
+    (gid / n, (gid % n, ()))
+    (acc eC (gid / n, (gid % n, ())))
 
 unfold
 let kpost
@@ -42,18 +57,18 @@ let kpost
   (comb : binop et)
   (comb_r : binop real { comb `approx2` comb_r })
   (#m #n #k : nat)
-  (#lA : M.layout m k)
-  (#lB : M.layout k n)
-  (#lC : M.layout m n)
-  (gA : M.array2 et lA)
-  (gB : M.array2 et lB)
-  (gC : M.array2 et lC)
-  (eA : ematrix et m k)
-  (eB : ematrix et k n)
-  (eC : ematrix et m n)
-  (rA : ematrix real m k{eA %~ rA})
-  (rB : ematrix real k n{eB %~ rB})
-  (rC : ematrix real m n{eC %~ rC})
+  (#lA : layout2 m k)
+  (#lB : layout2 k n)
+  (#lC : layout2 m n)
+  (gA : tensor et lA)
+  (gB : tensor et lB)
+  (gC : tensor et lC)
+  (eA : chest2 et m k)
+  (eB : chest2 et k n)
+  (eC : chest2 et m n)
+  (rA : chest2 real m k{eA %~ rA})
+  (rB : chest2 real k n{eB %~ rB})
+  (rC : chest2 real m n{eC %~ rC})
   (fA fB : perm)
   (gid : natlt (m * n))
   : slprop
@@ -61,28 +76,30 @@ let kpost
   gA |-> Frac (fA /. (m * n)) eA **
   gB |-> Frac (fB /. (m * n)) eB **
   exists* v.
-    M.pts_to_cell gC (gid / n, gid % n) v **
+    pts_to_cell gC (gid / n, (gid % n, ())) v **
       pure (v %~ MS.gemm_single comb_r rA rB rC (gid / n) (gid % n))
+
+#set-options "--split_queries always"
 
 inline_for_extraction noextract
 fn kf
   (#et : Type0) {| floating et, real_like et, floating_real_like et |}
   (comb : binop et)
   (comb_r : binop real { comb `approx2` comb_r })
-  (#m #n #k : szp)
-  (#lA : M.layout m k)
-  (#lB : M.layout k n)
-  (#lC : M.layout m n)
-  {| cA : T.ctlayout lA, cB : T.ctlayout lB, cC : T.ctlayout lC |}
-  (gA : M.array2 et lA)
-  (gB : M.array2 et lB)
-  (gC : M.array2 et lC)
-  (eA : ematrix et m k)
-  (eB : ematrix et k n)
-  (eC : ematrix et m n)
-  (rA : ematrix real m k{eA %~ rA})
-  (rB : ematrix real k n{eB %~ rB})
-  (rC : ematrix real m n{eC %~ rC})
+  (#m #n #k : SZ.t)
+  (#lA : layout2 m k)
+  (#lB : layout2 k n)
+  (#lC : layout2 m n)
+  {| ctlayout lA, ctlayout lB, ctlayout lC |}
+  (gA : tensor et lA)
+  (gB : tensor et lB)
+  (gC : tensor et lC)
+  (eA : chest2 et m k)
+  (eB : chest2 et k n)
+  (eC : chest2 et m n)
+  (rA : chest2 real m k{eA %~ rA})
+  (rB : chest2 real k n{eB %~ rB})
+  (rC : chest2 real m n{eC %~ rC})
   (fA fB : perm)
   (gid : szlt (m *^ n))
   ()
@@ -94,14 +111,14 @@ fn kf
     gpu **
     kpost comb comb_r gA gB gC eA eB eC rA rB rC fA fB gid
 {
-  let trow = gid /^ n; assert (rewrites_to trow (gid /^ n));
-  let tcol = gid %^ n; assert (rewrites_to tcol (gid %^ n));
+  let trow : szlt m = gid /^ n; assert (rewrites_to trow (gid /^ n));
+  let tcol : szlt n = gid %^ n; assert (rewrites_to tcol (gid %^ n));
 
-  let s = Kuiper.DotProd.matmul_kahan_dotprod gA gB trow tcol rA rB;
+  let s = Kuiper.DotProd.matmul_kahan_dotprod_t gA gB trow tcol rA rB;
 
-  let v0 = M.read_cell' gC trow tcol;
+  let v0 = tensor_read_cell gC (trow, (tcol, ()));
   let v1 = comb v0 s;
-  M.write_cell' gC trow tcol v1;
+  tensor_write_cell gC (trow, (tcol, ())) v1;
 
   ()
 }
@@ -112,19 +129,19 @@ fn setup
   (comb : binop et)
   (comb_r : binop real { comb `approx2` comb_r })
   (#m #n #k : szp)
-  (#lA : M.layout m k)
-  (#lB : M.layout k n)
-  (#lC : M.layout m n)
-  {| T.ctlayout lA, T.ctlayout lB, T.ctlayout lC |}
-  (gA : M.array2 et lA)
-  (gB : M.array2 et lB)
-  (gC : M.array2 et lC)
-  (eA : ematrix et m k)
-  (eB : ematrix et k n)
-  (eC : ematrix et m n)
-  (rA : ematrix real m k{eA %~ rA})
-  (rB : ematrix real k n{eB %~ rB})
-  (rC : ematrix real m n{eC %~ rC})
+  (#lA : layout2 m k)
+  (#lB : layout2 k n)
+  (#lC : layout2 m n)
+  {| ctlayout lA, ctlayout lB, ctlayout lC |}
+  (gA : tensor et lA)
+  (gB : tensor et lB)
+  (gC : tensor et lC)
+  (eA : chest2 et m k)
+  (eB : chest2 et k n)
+  (eC : chest2 et m n)
+  (rA : chest2 real m k{eA %~ rA})
+  (rB : chest2 real k n{eB %~ rB})
+  (rC : chest2 real m n{eC %~ rC})
   (fA fB : perm)
   ()
   norewrite
@@ -137,18 +154,24 @@ fn setup
       kpre comb comb_r gA gB gC eA eB eC rA rB rC fA fB gid) **
     emp (* frame *)
 {
-  M.share_n gA (m *^ n);
-  M.share_n gB (m *^ n);
+  // Sharing the input matrices (splitting permissions)
+  tensor_share_n gA (m *^ n);
+  tensor_share_n gB (m *^ n);
 
-  M.explode gC;
-  forevery_rw_type (M.ait m n) (natlt m & natlt n) _;
+  // Sharing the output matrix (splitting each cell)
+  tensor_explode gC;
+  forevery_iso (abs_bij #m #n) _;
+  forevery_ext _ (fun (ij : natlt m & natlt n) ->
+    pts_to_cell gC (fst ij, (snd ij, ())) (acc eC (fst ij, (snd ij, ()))));
   forevery_unflatten' _;
-  forevery_unfactor' (m *^ n) m n (fun r c ->
-    M.pts_to_cell gC (r, c) (macc eC r c));
 
+  forevery_unfactor' (m *^ n) m n (fun r c ->
+    pts_to_cell gC (r, (c, ())) (acc eC (r, (c, ()))));
+
+  // Join resources into a single bigstar
   forevery_zip #(natlt2 m n)
     (fun _ -> gB |-> Frac (fB /. (m *^ n)) eB)
-    (fun i -> M.pts_to_cell gC ((i/n <: natlt m), (i%n <: natlt n)) (macc eC (i/n) (i%n)));
+    (fun i -> pts_to_cell gC ((i/n <: natlt m), ((i%n <: natlt n), ())) (acc eC ((i/n <: natlt m), ((i%n <: natlt n), ()))));
   forevery_zip #(natlt2 m n)
     (fun _ -> gA |-> Frac (fA /. (m *^ n)) eA)
     _;
@@ -163,19 +186,19 @@ fn teardown
   (comb : binop et)
   (comb_r : binop real { comb `approx2` comb_r })
   (#m #n #k : szp)
-  (#lA : M.layout m k)
-  (#lB : M.layout k n)
-  (#lC : M.layout m n)
-  {| T.ctlayout lA, T.ctlayout lB, T.ctlayout lC |}
-  (gA : M.array2 et lA)
-  (gB : M.array2 et lB)
-  (gC : M.array2 et lC)
-  (eA : ematrix et m k)
-  (eB : ematrix et k n)
-  (eC : ematrix et m n)
-  (rA : ematrix real m k{eA %~ rA})
-  (rB : ematrix real k n{eB %~ rB})
-  (rC : ematrix real m n{eC %~ rC})
+  (#lA : layout2 m k)
+  (#lB : layout2 k n)
+  (#lC : layout2 m n)
+  {| ctlayout lA, ctlayout lB, ctlayout lC |}
+  (gA : tensor et lA)
+  (gB : tensor et lB)
+  (gC : tensor et lC)
+  (eA : chest2 et m k)
+  (eB : chest2 et k n)
+  (eC : chest2 et m n)
+  (rA : chest2 real m k{eA %~ rA})
+  (rB : chest2 real k n{eB %~ rB})
+  (rC : chest2 real m n{eC %~ rC})
   (fA fB : perm)
   ()
   norewrite
@@ -186,7 +209,7 @@ fn teardown
   ensures
     gA |-> Frac fA eA **
     gB |-> Frac fB eB **
-    (exists* (eC : ematrix et m n).
+    (exists* (eC : chest2 et m n).
       gC |-> eC ** pure (eC %~ MS.mmcomb comb_r rC rA rB))
 {
   forevery_unzip3
@@ -195,41 +218,62 @@ fn teardown
     _;
 
   forevery_rw_type (natlt (m *^ n)) (natlt (m * n))
-    (fun _ -> M.pts_to #et gA #(fA /. (v m * v n)) eA);
+    (fun _ -> gA |-> Frac (fA /. (v m * v n)) eA);
   forevery_rw_type (natlt (m *^ n)) (natlt (m * n))
-    (fun _ -> M.pts_to #et gB #(fB /. (v m * v n)) eB);
+    (fun _ -> gB |-> Frac (fB /. (v m * v n)) eB);
 
-  M.gather_n gA _;
-  M.gather_n gB _;
+  tensor_gather_n gA _;
+  tensor_gather_n gB _;
 
   forevery_factor (m *^ n) m n _;
+
   let vf = forevery_exists_2 #(natlt m) #_ #(natlt n) _;
 
+  (* need to use ext to get rid of the [(r*n+c)/n] arithmetic *)
+  assert (pure (forall (r c : nat). c < n ==> (r * n + c) / n == r));
+  assert (pure (forall (r c : nat). c < n ==> (r * n + c) % n == c));
   forevery_ext_2 _
     (fun (r : natlt m) (c : natlt n) ->
-      M.pts_to_cell gC (r, c) (vf r c) **
+      pts_to_cell gC (r, (c, ())) (vf r c) **
         pure (vf r c %~ MS.gemm_single comb_r rA rB rC r c));
 
   forevery_extract_pure_2
     (fun (r : natlt m) (c : natlt n) ->
-      M.pts_to_cell gC (r, c) (vf r c) **
+      pts_to_cell gC (r, (c, ())) (vf r c) **
         pure (vf r c %~ MS.gemm_single comb_r rA rB rC r c))
     (fun (r : natlt m) (c : natlt n) ->
       vf r c %~ MS.gemm_single comb_r rA rB rC r c)
     fn r c { (); };
 
-  let eC' : ematrix et m n = mkM (fun (r : natlt m) (c : natlt n) -> vf r c);
-  forevery_map_2
+  let eC' : chest2 et m n = mkM (fun (r : natlt m) (c : natlt n) -> vf r c);
+
+  ghost
+  fn aux (r:natlt m) (c:natlt n)
+    requires
+      pts_to_cell gC (r, (c, ())) (vf r c) **
+        pure (vf r c %~ MS.gemm_single comb_r rA rB rC r c)
+    ensures
+      pts_to_cell gC (r, (c, ())) (acc eC' (r, (c, ())))
+  {
+    assert (pure (macc eC' r c == vf r c));
+    ()
+  };
+  forevery_map_2 #(natlt m) #(natlt n)
     (fun (r : natlt m) (c : natlt n) ->
-      M.pts_to_cell gC (r, c) (vf r c) **
+      pts_to_cell gC (r, (c, ())) (vf r c) **
         pure (vf r c %~ MS.gemm_single comb_r rA rB rC r c))
     (fun (r : natlt m) (c : natlt n) ->
-      M.pts_to_cell gC (r, c) (macc eC' r c))
-    fn r c { () };
+      pts_to_cell gC (r, (c, ())) (acc eC' (r, (c, ()))))
+    aux;
 
   forevery_flatten' (fun (rc : natlt m & natlt n) ->
-    M.pts_to_cell gC rc (macc eC' (fst rc) (snd rc)));
-  M.implode gC;
+    pts_to_cell gC (fst rc, (snd rc, ())) (acc eC' (fst rc, (snd rc, ()))));
+
+  forevery_iso (bij_sym (abs_bij #m #n)) _;
+  forevery_ext _ (fun (i : abs (m @| n @| INil)) ->
+    pts_to_cell gC i (acc eC' i));
+  tensor_implode gC;
+
   assert (pure (eC' %~ MS.mmcomb comb_r rC rA rB));
   ();
 }
@@ -240,22 +284,22 @@ let kdesc
   (comb : binop et)
   (comb_r : binop real { comb `approx2` comb_r })
   (#m #n #k : szp)
-  (#lA : M.layout m k)
-  (#lB : M.layout k n)
-  (#lC : M.layout m n)
-  {| T.ctlayout lA, T.ctlayout lB, T.ctlayout lC |}
-  (gA : M.array2 et lA { M.is_global gA })
-  (gB : M.array2 et lB { M.is_global gB })
-  (gC : M.array2 et lC { M.is_global gC })
-  (#eA #eB #eC : ematrix et _ _)
-  (rA : ematrix real m k{eA %~ rA})
-  (rB : ematrix real k n{eB %~ rB})
-  (rC : ematrix real m n{eC %~ rC})
+  (#lA : layout2 m k)
+  (#lB : layout2 k n)
+  (#lC : layout2 m n)
+  {| ctlayout lA, ctlayout lB, ctlayout lC |}
+  (gA : tensor et lA { is_global gA })
+  (gB : tensor et lB { is_global gB })
+  (gC : tensor et lC { is_global gC })
+  (#eA #eB #eC : chest2 et _ _)
+  (rA : chest2 real m k{eA %~ rA})
+  (rB : chest2 real k n{eB %~ rB})
+  (rC : chest2 real m n{eC %~ rC})
   (#fA #fB : perm)
   (#_ : squash (size_req m n k))
   : kernel_desc
     (gA |-> Frac fA eA ** gB |-> Frac fB eB ** gC |-> eC)
-    (gA |-> Frac fA eA ** gB |-> Frac fB eB ** (exists* (eC : ematrix et m n). gC |-> eC ** pure (eC %~ MS.mmcomb comb_r rC rA rB)))
+    (gA |-> Frac fA eA ** gB |-> Frac fB eB ** (exists* (eC : chest2 et m n). gC |-> eC ** pure (eC %~ MS.mmcomb comb_r rC rA rB)))
 =
 {
   nthr     = m *^ n;
@@ -275,30 +319,29 @@ fn mmcomb_gpu_approx
   (comb : binop et)
   (comb_r : binop real { approx2 comb comb_r })
   (#m #n #k : szp)
-  (#lA : M.layout m k)
-  (#lB : M.layout k n)
-  (#lC : M.layout m n)
-  {| T.ctlayout lA, T.ctlayout lB, T.ctlayout lC |}
-  (gA : M.array2 et lA { M.is_global gA })
-  (gB : M.array2 et lB { M.is_global gB })
-  (gC : M.array2 et lC { M.is_global gC })
-  (#eA : ematrix et m k)
-  (#eB : ematrix et k n)
-  (#eC : ematrix et m n)
-  (rA : ematrix real m k)
-  (rB : ematrix real k n)
-  (rC : ematrix real m n)
+  (#lA : layout2 m k)
+  (#lB : layout2 k n)
+  (#lC : layout2 m n)
+  {| ctlayout lA, ctlayout lB, ctlayout lC |}
+  (gA : tensor et lA { is_global gA })
+  (gB : tensor et lB { is_global gB })
+  (gC : tensor et lC { is_global gC })
+  (#eA : chest2 et m k)
+  (#eB : chest2 et k n)
+  (#eC : chest2 et m n)
+  (rA : chest2 real m k)
+  (rB : chest2 real k n)
+  (rC : chest2 real m n)
   (#fA #fB : perm)
   norewrite
   preserves
-    cpu **
-    on gpu_loc (gA |-> Frac fA eA ** gB |-> Frac fB eB)
+    cpu ** on gpu_loc (gA |-> Frac fA eA ** gB |-> Frac fB eB)
   requires
     pure (size_req m n k) **
     pure (eA %~ rA /\ eB %~ rB /\ eC %~ rC) **
     on gpu_loc (gC |-> eC)
   ensures
-    exists* (eC' : ematrix et m n).
+    exists* (eC' : chest2 et m n).
       on gpu_loc (gC |-> eC') **
       pure (eC' %~ MS.mmcomb comb_r rC rA rB)
 {
