src/lib/ghost/Kuiper.Ghost.TensorTranspose.fst
@@ -4,12 +4,9 @@ module Kuiper.Ghost.TensorTranspose
 
 open Kuiper
 open Kuiper.Tensor
-open Kuiper.Array2
 open Kuiper.EMatrix
 open Kuiper.Tensor.Layout.Alg
-
 open Kuiper.Injection
-
 
 // Not great that we need these helpers.
 #push-options "--fuel 2 --ifuel 2 --z3rlimit 80"
@@ -31,20 +28,20 @@ ghost
 fn ghost_transpose1
   (#et:Type)
   (#rows #cols : nat)
-  (gA : array2 et (l2_row_major rows cols))
+  (gA : tensor et (l2_row_major rows cols))
   (#m : ematrix et rows cols)
   requires
     gA |-> m
   ensures
     row2col gA |-> mtranspose m
 {
-  lower gA;
+  tensor_concr gA;
   assert (pure (Seq.equal
                   (to_seq (l2_row_major rows cols) m)
                   (to_seq (l2_col_major cols rows) (mtranspose m))));
   rewrite core gA |-> to_seq (l2_row_major rows cols) m
        as core gA |-> to_seq (l2_col_major cols rows) (mtranspose m);
-  raise (l2_col_major cols rows) (core gA);
+  tensor_abs (l2_col_major cols rows) (core gA);
 }
 #pop-options
 
@@ -53,20 +50,20 @@ ghost
 fn ghost_transpose2
   (#et:Type)
   (#rows #cols : nat)
-  (gA : array2 et (l2_col_major rows cols))
+  (gA : tensor et (l2_col_major rows cols))
   (#m : ematrix et rows cols)
   requires
     gA |-> m
   ensures
     col2row gA |-> mtranspose m
 {
-  lower gA;
+  tensor_concr gA;
   assert (pure (Seq.equal
                   (to_seq (l2_col_major rows cols) m)
                   (to_seq (l2_row_major cols rows) (mtranspose m))));
   rewrite core gA |-> to_seq (l2_col_major rows cols) m
        as core gA |-> to_seq (l2_row_major cols rows) (mtranspose m);
-  raise (l2_row_major cols rows) (core gA);
+  tensor_abs (l2_row_major cols rows) (core gA);
 }
 #pop-options
 
@@ -74,7 +71,7 @@ ghost
 fn ghost_transpose1_back
   (#et:Type)
   (#rows #cols : nat)
-  (gA : array2 et (l2_row_major rows cols))
+  (gA : tensor et (l2_row_major rows cols))
   (#m : ematrix et cols rows)
   requires
     row2col gA |-> m
@@ -93,7 +90,7 @@ ghost
 fn ghost_transpose2_back
   (#et:Type)
   (#rows #cols : nat)
-  (gA : array2 et (l2_col_major rows cols))
+  (gA : tensor et (l2_col_major rows cols))
   (#m : ematrix et cols rows)
   requires
     col2row gA |-> m
