src/lib/ghost/Kuiper.Ghost.TensorTranspose.fsti
@@ -3,7 +3,7 @@ module Kuiper.Ghost.TensorTranspose
 #lang-pulse
 
 open Kuiper
-open Kuiper.Array2
+open Kuiper.Tensor
 open Kuiper.EMatrix
 open Kuiper.Tensor.Layout.Alg
 
@@ -11,23 +11,23 @@ unfold
 let row2col
   (#et : Type)
   (#rows #cols : erased nat)
-  (m : array2 et (l2_row_major rows cols))
-  : array2 et (l2_col_major cols rows) =
+  (m : tensor et (l2_row_major rows cols))
+  : tensor et (l2_col_major cols rows) =
   from_array (l2_col_major cols rows) (core m)
 
 unfold
 let col2row
   (#et : Type)
   (#rows #cols : erased nat)
-  (m : array2 et (l2_col_major rows cols))
-  : array2 et (l2_row_major cols rows) =
+  (m : tensor et (l2_col_major rows cols))
+  : tensor et (l2_row_major cols rows) =
   from_array (l2_row_major cols rows) (core m)
 
 ghost
 fn ghost_transpose1
   (#et:Type)
   (#rows #cols : nat)
-  (gA : array2 et (l2_row_major rows cols))
+  (gA : tensor et (l2_row_major rows cols))
   (#m : ematrix et rows cols)
   requires
     gA |-> m
@@ -38,7 +38,7 @@ ghost
 fn ghost_transpose2
   (#et:Type)
   (#rows #cols : nat)
-  (gA : array2 et (l2_col_major rows cols))
+  (gA : tensor et (l2_col_major rows cols))
   (#m : ematrix et rows cols)
   requires
     gA |-> m
@@ -49,7 +49,7 @@ ghost
 fn ghost_transpose1_back
   (#et:Type)
   (#rows #cols : nat)
-  (gA : array2 et (l2_row_major rows cols))
+  (gA : tensor et (l2_row_major rows cols))
   (#m : ematrix et cols rows)
   requires
     row2col gA |-> m
@@ -60,7 +60,7 @@ ghost
 fn ghost_transpose2_back
   (#et:Type)
   (#rows #cols : nat)
-  (gA : array2 et (l2_col_major rows cols))
+  (gA : tensor et (l2_col_major rows cols))
   (#m : ematrix et cols rows)
   requires
     col2row gA |-> m
