src/lib/kernel/gemm/Kuiper.Kernel.GEMM.Naive2.fsti
@@ -1,13 +1,17 @@
 module Kuiper.Kernel.GEMM.Naive2
 
-(* This is a less naive matmul. It spawns full blocks of 1024 threads,
-going in row major order through the output matrix and with each thread
-computing a full dot product. *)
+(* Like Naive, but spawns full blocks of threads going in row-major order
+through the output matrix, with each thread computing a full dot product.
+Tensor analog of Naive2. *)
 
 #lang-pulse
 
 open Kuiper
 
+module MS = Kuiper.Spec.GEMM
+open Kuiper.Tensor
+open Kuiper.Index
+open Kuiper.Chest
 open Kuiper.Kernel.GEMMGPU.Type
 
 inline_for_extraction noextract
@@ -15,7 +19,56 @@ let size_req : size_req_t =
   fun m n k -> m * n <= max_blocks * max_threads
 
 inline_for_extraction noextract
-val mmcomb_gpu_exact : matmulcomb_gpu_ty size_req
+fn mmcomb_gpu_exact
+  (#et : Type0) {| scalar et |}
+  (comb : binop et)
+  (#m #n #k : szp)
+  (#lA : layout2 m k)
+  (#lB : layout2 k n)
+  (#lC : layout2 m n)
+  {| ctlayout lA, ctlayout lB, ctlayout lC |}
+  (gA : tensor et lA { is_global gA })
+  (gB : tensor et lB { is_global gB })
+  (gC : tensor et lC { is_global gC })
+  (#eA #eB #eC : chest2 et _ _)
+  (#fA #fB : perm)
+  norewrite
+  preserves
+    cpu ** on gpu_loc (gA |-> Frac fA eA ** gB |-> Frac fB eB)
+  requires
+    pure (size_req m n k) **
+    on gpu_loc (gC |-> eC)
+  ensures
+    on gpu_loc (gC |-> MS.mmcomb comb eC eA eB)
 
 inline_for_extraction noextract
-val mmcomb_gpu_approx : matmulcomb_gpu_approx_ty size_req
+fn mmcomb_gpu_approx
+  (#et : Type0) {| scalar et, real_like et |}
+  (comb : binop et)
+  (comb_r : binop real { comb `approx2` comb_r })
+  (#m #n #k : szp)
+  (#lA : layout2 m k)
+  (#lB : layout2 k n)
+  (#lC : layout2 m n)
+  {| ctlayout lA, ctlayout lB, ctlayout lC |}
+  (gA : tensor et lA { is_global gA })
+  (gB : tensor et lB { is_global gB })
+  (gC : tensor et lC { is_global gC })
+  (#eA : chest2 et m k)
+  (#eB : chest2 et k n)
+  (#eC : chest2 et m n)
+  (rA : chest2 real m k)
+  (rB : chest2 real k n)
+  (rC : chest2 real m n)
+  (#fA #fB : perm)
+  norewrite
+  preserves
+    cpu ** on gpu_loc (gA |-> Frac fA eA ** gB |-> Frac fB eB)
+  requires
+    pure (size_req m n k) **
+    pure (eA %~ rA /\ eB %~ rB /\ eC %~ rC) **
+    on gpu_loc (gC |-> eC)
+  ensures
+    exists* (eC' : chest2 et m n).
+      on gpu_loc (gC |-> eC') **
+      pure (eC' %~ MS.mmcomb comb_r rC rA rB)
